# 풀이

```js
function solution(sequence, k) {
  const len = sequence.length;
  let answer = [0, len];
  let sum = sequence[0];
  let start = 0;

  for (let i = 0; i < len; i++) {
    let cur = sequence[i];
    sum += sequence[i + 1];

    if (cur > k) break;

    if (cur === k) {
      answer[0] = i;
      answer[1] = i;
      break;
    }

    if (sum === k && answer[1] - answer[0] > i + 1 - start) {
      answer[0] = start;
      answer[1] = i + 1;
    }

    if (sum > k) {
      while (true) {
        if (sum < k) break;
        if (sum === k && answer[1] - answer[0] > i + 1 - start) {
          answer[0] = start;
          answer[1] = i + 1;
        }
        sum -= sequence[start];
        start++;
      }
    }
  }
  return answer;
}
```
